src/Language/PlutusIR/Semantics/SemanticEquivalence/CompatibilityLemmas/Apply.v
@@ -3,40 +3,171 @@ Import NamedTerm.
 Require Import PlutusCert.Language.PlutusIR.Semantics.Dynamic.
 Require Import PlutusCert.Language.PlutusIR.Semantics.Static.
 Require Import PlutusCert.Language.PlutusIR.Semantics.TypeSafety.Preservation.
-Require Import PlutusCert.Language.PlutusIR.Semantics.TypeSafety.SubstitutionPreservesTyping.
-Require Import PlutusCert.Language.PlutusIR.Semantics.SemanticEquivalence.Def.
+Require Import PlutusCert.Language.PlutusIR.Semantics.SemanticEquivalence.LogicalRelation.RelationalModel.
 Require Import PlutusCert.Language.PlutusIR.Semantics.SemanticEquivalence.Monotonicity.
 Require Import PlutusCert.Language.PlutusIR.Semantics.SemanticEquivalence.ReductionInvariance.
-Require Import PlutusCert.Language.PlutusIR.Semantics.SemanticEquivalence.Termination.
 
 Require Import Arith.
 Require Import Coq.Logic.Decidable.
 
 
-
-Lemma RC_compatibility_Apply : forall k rho T1 T2 e1 e2 e1' e2',
-    RC k rho (Ty_Fun T1 T2) e1 e1' ->
-    RC k rho T1 e2 e2' ->
-    RC k rho T2 (Apply e1 e2) (Apply e1' e2').
+Lemma msubst_Apply : forall ss t1 t2 t',
+    msubst ss (Apply t1 t2) t' ->
+    exists t1' t2', msubst ss t1 t1' /\ msubst ss t2 t2' /\ t' = (Apply t1' t2').
 Proof.
-  intros k rho T1 T2 e1 e2 e1' e2'.
-  intros RC1 RC2.
+  induction ss; intros.
+  - inversion H. subst.
+    exists t1, t2.
+    eauto using msubst_nil, msubst_cons. 
+  - inversion H. subst.
+    rename t'0 into t''.
+    inversion H2. subst.
+    apply IHss in H5.
+    destruct H5 as [t1'' [t2'' [H9 [H10 H11]]]].
+    exists t1'', t2''.
+    split. {
+      apply msubst_cons with t1'.
+      + assumption.
+      + apply H9.
+    }
+    split. {
+      apply msubst_cons with t2'.
+      + assumption.
+      + apply H10.
+    }
+    assumption.
+Qed.
 
-  assert (Htyp : emptyContext |-+ (Apply e1 e2) : (apply_tysubsts_1 rho T2)). {
-    apply T_Apply with T1.
-    - eapply RC_typable_empty_1; eauto.
-    - eapply RC_typable_empty_1; eauto.
-  } 
-  assert (Htyp' : emptyContext |-+ (Apply e1' e2') : (apply_tysubsts_2 rho T2)). {
-    apply T_Apply with T1.
-    - eapply RC_typable_empty_2; eauto.
-    - eapply RC_typable_empty_2; eauto.
+Lemma msubstA_Apply : forall ss t1 t2 t',
+    msubstA ss (Apply t1 t2) t' ->
+    exists t1' t2', msubstA ss t1 t1' /\ msubstA ss t2 t2' /\ t' = (Apply t1' t2').
+Proof.
+  induction ss; intros.
+  - inversion H. subst.
+    exists t1, t2.
+    eauto using msubstA_nil, msubstA_cons. 
+  - inversion H. subst.
+    rename t'0 into t''.
+    inversion H2. subst.
+    apply IHss in H5.
+    destruct H5 as [t1'' [t2'' [H9 [H10 H11]]]].
+    exists t1'', t2''.
+    split. {
+      apply msubstA_cons with t1'.
+      + assumption.
+      + apply H9.
+    }
+    split. {
+      apply msubstA_cons with t2'.
+      + assumption.
+      + apply H10.
+    }
+    assumption.
+Qed.
+
+Lemma inspect_eval__Apply1 : forall t1 t2 j v0,
+    Apply t1 t2 =[j]=> v0 ->
+    exists j1 v1, t1 =[j1]=> v1 /\ j1 <= j.
+Proof.
+  intros.
+  inversion H. all: subst.
+  - exists k1.
+    exists (LamAbs x T t4).
+    split; auto.
+Admitted.
+
+Lemma inspect_eval__Apply2 : forall t1 t2 j v0 j1 v1,
+    Apply t1 t2 =[j]=> v0 ->
+    terminates_incl t1 j1 v1 j ->
+    exists j2 v2, terminates_incl t2 j2 v2 (j - j1).
+Proof. 
+  intros. 
+  destruct H0.
+  inversion H.
+  all: subst.
+  - assert (v1 = LamAbs x T t4 /\ j1 = k1) by (eapply eval__deterministic; eauto).
+    destruct H2. subst.
+    exists k2.
+    
+    exists v2.
+    split; auto.
+Admitted.
+
+Lemma inspect_eval__Apply3 : forall t1 t2 j v0 j1 x T t0 j2 v2 t0',
+    Apply t1 t2 =[j]=> v0 ->
+    terminates_incl t1 j1 (LamAbs x T t0) j ->
+    terminates_incl t2 j2 v2 (j - j1) ->
+    substitute x v2 t0 t0' ->
+    exists j0, terminates_incl t0' j0 v0 (j - j1 - j2 - 1) /\ j = j1 + j2 + 1 + j0.
+Proof. 
+  intros. 
+  destruct H0.
+  destruct H1.
+  inversion H.
+  all: subst.
+  - assert (LamAbs x0 T0 t5 = LamAbs x T t0 /\ k1 = j1) by (eapply eval__deterministic; eauto).
+    destruct H5. inversion H5. subst.
+    assert (v1 = v2 /\ k2 = j2) by (eapply eval__deterministic; eauto).
+    destruct H6. subst.
+    assert (t0'0 = t0') by (eapply substitute__deterministic; eauto).
+    subst.
+    exists k0.
+    split; auto.
+    split; auto.
+Admitted.
+
+Lemma compatibility_Apply : forall Delta Gamma e1 e2 e1' e2' T1 T2 ,
+    LR_logically_approximate Delta Gamma e1 e1' (Ty_Fun T1 T2) ->
+    LR_logically_approximate Delta Gamma e2 e2' T1 ->
+    LR_logically_approximate Delta Gamma (Apply e1 e2) (Apply e1' e2') T2.
+Proof.
+  intros Delta Gamma e1 e2 e1' e2' T1 T2 IH_LR1 IH_LR2.
+  unfold LR_logically_approximate.
+
+  split. {
+    edestruct IH_LR1 as [Htyp__e1 [Htyp__e1' H1]].
+    edestruct IH_LR2 as [Htyp__e2 [Htyp__e2' H2]].
+    eapply T_Apply. eauto. eauto.
   }
 
-  autorewrite with RC.
+  split. {
+    edestruct IH_LR1 as [Htyp__e1 [Htyp__e1' H1]].
+    edestruct IH_LR2 as [Htyp__e2 [Htyp__e2' H2]].
+    eapply T_Apply. eauto. eauto.
+  }
 
-  (* First part of the proof *)
-  split; auto. split; auto.
+  intros k rho env env' ct ck HeqDelta HeqGamma [H_RD H_RG].
+  subst.
+
+  intros e_msa e'_msa e_ms e'_ms.
+  intros HmsA__e_msa HmsA__e'_msa Hms__e_ms Hms__e'_ms.
+
+  destruct (msubstA_Apply _ _ _ _ HmsA__e_msa) as [e1_msa [e2_msa [HmsA__e1_msa [HmsA__e2_msa Heq]]]].
+  destruct (msubstA_Apply _ _ _ _ HmsA__e'_msa) as [e1'_msa [e2'_msa [HmsA__e1'_msa [HmsA__e2'_msa Heq']]]].
+  subst.
+  destruct (msubst_Apply _ _ _ _ Hms__e_ms) as [e1_ms [e2_ms [Hms__e1_ms [Hms__e2_ms Heq]]]].
+  destruct (msubst_Apply _ _ _ _ Hms__e'_ms) as [e1'_ms [e2'_ms [Hms__e1'_ms [Hms__e2'_ms Heq']]]].
+  subst.
+
+  autorewrite with RC.
+  split. {
+    replace emptyContext with (@empty Kind, mupd (msyn1 rho) empty).
+    - eapply msubst_preserves_typing_1; eauto.
+      eapply msubstA_preserves_typing_1; eauto.
+      destruct IH_LR1.
+      destruct IH_LR2.
+      eauto with typing.
+    - rewrite mupd_empty. reflexivity.
+  }
+  split. {
+    replace emptyContext with (@empty Kind, mupd (msyn2 rho) empty).
+    - eapply msubst_preserves_typing_2; eauto.
+      eapply msubstA_preserves_typing_2; eauto.
+      destruct IH_LR1. destruct H0.
+      destruct IH_LR2. destruct H3.
+      eauto with typing.
+    - rewrite mupd_empty. reflexivity.
+  }
 
   (* Second part of the proof *)
 
@@ -53,7 +184,7 @@ Proof.
       # e1 =[j1]=> e_f1, and
       # j1 <= j
   *)
-  assert (temp: exists j1 e_f1, e1 =[j1]=> e_f1 /\ j1 <= j) by eauto using termination_congr_Apply1.
+  assert (temp: exists j1 e_f1, e1_ms =[j1]=> e_f1 /\ j1 <= j) by eauto using inspect_eval__Apply1.
   destruct temp as [j1 [e_f1 [Hev__e1 Hle__j1_j]]].
 
   (** 
@@ -63,6 +194,8 @@ Proof.
   *)
   assert (Hlt__j1_k : j1 < k) by eauto using Nat.le_lt_trans. 
 
+  unfold LR_logically_approximate in IH_LR1.
+  assert (RC1 : RC k (Ty_Fun T1 T2) rho e1_ms e1'_ms) by (eapply IH_LR1; eauto).
   autorewrite with RC in RC1.
   destruct RC1 as [_ [_ RC1]].
   remember (RC1 j1 Hlt__j1_k e_f1 Hev__e1) as temp.
@@ -83,9 +216,9 @@ Proof.
       TODO: This is not actually true because of the way we handle builtin functions. However,
       I will assume this for now to simplify the proof.
   *)
-  assert (temp: exists x e_f11, e_f1 = LamAbs x T1 e_f11). { apply skip. }
+  assert (temp: exists x e_f11, e_f1 = LamAbs x (msubstT (msyn1 rho) T1) e_f11). { apply skip. }
   destruct temp as [x [e_f11 Heq]].
-  assert (temp: exists x' e'_f11, e'_f1 = LamAbs x' T1 e'_f11). { apply skip. }
+  assert (temp: exists x' e'_f11, e'_f1 = LamAbs x' (msubstT (msyn2 rho) T1) e'_f11). { apply skip. }
   destruct temp as [x' [e'_f11 Heq']].
   
   (**
@@ -97,16 +230,18 @@ Proof.
       # e2 =[j2]=> e_f2, and
       # j2 <= j - j1
   *)
-  assert (temp: exists j2 e_f2, e2 =[j2]=> e_f2 /\ j2 <= j - j1). {
-    eapply termination_congr_Apply2; eauto. split; eauto.
+  assert (temp: exists j2 e_f2, e2_ms =[j2]=> e_f2 /\ j2 <= j - j1). {
+    eapply inspect_eval__Apply2; eauto. split; eauto.
   }
   destruct temp as [j2 [e_f2 [Hev__e2 Hle__j2]]].
 
   (**
       Instantiate the second conjunct of RC2 with (k - j1). 
   *)
+  unfold LR_logically_approximate in IH_LR2.
+  assert (RC2 : RC k T1 rho e2_ms e2'_ms) by (eapply IH_LR2; eauto).
   remember RC2 as RC2'. clear HeqRC2'.
-  assert (temp: RC (k - j1) rho T1 e2 e2'). {
+  assert (temp: RC (k - j1) T1 rho e2_ms e2'_ms). {
     eapply RC_monotone.
     - eassumption.
     - apply skip. (* TODO *) 
@@ -131,7 +266,7 @@ Proof.
       # (k - j1 - j2, e_f2, e'_f2) \in RV[[T1]]
   *)
   destruct RC2 as [e'_f2 [j'_2 [Hev__e2' _]]].
-  assert (RV2: RC (k - j1 - j2) rho T1 e_f2 e'_f2). {
+  assert (RV2: RC (k - j1 - j2) T1 rho e_f2 e'_f2). {
     apply skip. (* TODO *)
   }
 
@@ -169,7 +304,7 @@ Proof.
   remember (RV1 x e_f11 x' e'_f11 Heq Heq' (k - j1 - j2 - 1) Hlt__j1_j2_k_j1) as temp.
   clear Heqtemp. clear RV1. rename temp into RV1.
 
-  assert (RC (k - j1 - j2 - 1) rho T1 v_f2 v'_f2). {
+  assert (RC (k - j1 - j2 - 1) T1 rho v_f2 v'_f2). {
     eapply RC_monotone.
     - eassumption.
     - apply skip.
@@ -184,7 +319,7 @@ Proof.
   }
   destruct temp as [e'_f11__s Hsubst'].
 
-  assert (RC (k - j1 - j2 - 1) rho T2 e_f11__s e'_f11__s). {
+  assert (RC (k - j1 - j2 - 1) T2 rho e_f11__s e'_f11__s). {
     eapply RV1; eauto.
     all: eauto using eval_value, eval_to_value.
   }
@@ -193,7 +328,7 @@ Proof.
   destruct H0 as [_ [_ H0]].
 
   assert (exists j0, terminates_incl e_f11__s j0 e_f (j - j1 - j2 - 1) /\ j = j1 + j2 + 1 + j0). {
-    eapply termination_congr_Apply3; eauto. split; eauto. subst. eauto. split; eauto.
+    eapply inspect_eval__Apply3; eauto. split; eauto. subst. eauto. split; eauto.
   }
   destruct H1 as [j3 H1]. destruct H1. destruct H1.
 
