src/Language/PlutusIR/Semantics/SemanticEquivalence/CompatibilityLemmas/Builtin.v
@@ -1,0 +1,79 @@
+Require Import PlutusCert.Language.PlutusIR.
+Import NamedTerm.
+Require Import PlutusCert.Language.PlutusIR.Semantics.Dynamic.
+Require Import PlutusCert.Language.PlutusIR.Semantics.Static.
+Require Import PlutusCert.Language.PlutusIR.Semantics.SemanticEquivalence.LogicalRelation.RelationalModel.
+
+Require Import Arith.
+
+Lemma msubst_Builtin : forall ss f t',
+    msubst ss (Builtin f) t' ->
+    t' = Builtin f.
+Proof. 
+  induction ss; intros.
+  - inversion H. subst.
+    reflexivity.
+  - inversion H. subst.
+    inversion H2. subst.
+    auto.
+Qed.
+
+Lemma msubstA_Builtin : forall ss f t',
+    msubstA ss (Builtin f) t' ->
+    t' = Builtin f.
+Proof.
+  induction ss; intros.
+  - inversion H. subst.
+    reflexivity.
+  - inversion H. subst.
+    inversion H2. subst.
+    auto.
+Qed.
+
+Lemma compatibility_Builtin: forall Delta Gamma f,
+    LR_logically_approximate Delta Gamma (Builtin f) (Builtin f) (lookupBuiltinTy f).
+Proof.
+  intros Delta Gamma f.
+  unfold LR_logically_approximate.
+
+  split. { apply T_Builtin. }
+  split. { apply T_Builtin. }
+  
+  intros k rho env env' ct ck HeqDelta HeqGamma [H_RD H_RG].
+  subst.
+
+  intros e_msa e'_msa e_ms e'_ms.
+  intros HmsA__e_msa HmsA__e'_msa Hms__e_ms Hms__e'_ms.
+
+  apply msubstA_Builtin in HmsA__e_msa as Heq.
+  apply msubstA_Builtin in HmsA__e'_msa as Heq'. 
+  subst.
+  apply msubst_Builtin in Hms__e_ms as Heq.
+  apply msubst_Builtin in Hms__e'_ms as Heq'.
+  subst.
+  
+  autorewrite with RC.
+  split. {
+    replace emptyContext with (@empty Kind, mupd (msyn1 rho) empty).
+    - eapply msubst_preserves_typing_1; eauto.
+      eapply msubstA_preserves_typing_1; eauto.
+      eauto with typing.
+    - rewrite mupd_empty. reflexivity.
+  }
+  split. {
+    replace emptyContext with (@empty Kind, mupd (msyn2 rho) empty).
+    - eapply msubst_preserves_typing_2; eauto.
+      eapply msubstA_preserves_typing_2; eauto.
+      eauto with typing.
+    - rewrite mupd_empty. reflexivity.
+  }
+
+  intros j Hlt__j e_f Hev__e_f.
+  inversion Hev__e_f. subst.
+  exists (Builtin f).
+  exists 0.
+  split. {
+    eapply E_Builtin.
+  }
+  destruct f; simpl; intros; discriminate. (* TODO *)
+Qed.
