src/Language/PlutusIR/Semantics/SemanticEquivalence/FundamentalProperty.v
@@ -7,7 +7,6 @@ Require Import PlutusCert.Language.PlutusIR.Semantics.TypeSafety.SubstitutionPre
 Require Import PlutusCert.Language.PlutusIR.Semantics.SemanticEquivalence.CompatibilityLemmas.
 Require Import PlutusCert.Language.PlutusIR.Semantics.SemanticEquivalence.LogicalRelation.RelationalModel.
 Require Import PlutusCert.Language.PlutusIR.Semantics.SemanticEquivalence.Monotonicity.
-Require Import PlutusCert.Language.PlutusIR.Semantics.SemanticEquivalence.Termination.
 
 
 (** ** The [R] Lemma *)
@@ -54,70 +53,18 @@ Proof.
   - intros. unfold P_has_type. intros. subst.
     apply skip.
 
-  - (* T_Apply *)
-    apply skip.
-    (*
-    intros Gamma t1 t2 T1 T2 Htyp_t1 IH_t1 Htyp_t2 IH_t2.
-    unfold P_has_type.
-    intros k c e1 e2 Heq Htyp _ V t3 t4 Hms_t3 Hms_t4.
-    subst.
-    
-    destruct (msubst_Apply _ _ _ _ Hms_t3) as [t3_1 [t3_2 [Hms_t3_1 [Hms_t3_2 Heq_t3]]]].
-    subst.
-    destruct (msubst_Apply _ _ _ _ Hms_t4) as [t4_1 [t4_2 [Hms_t4_1 [Hms_t4_2 Heq_t4]]]].
-    subst.
-
-    assert (emptyContext |-+ (Apply t3_1 t3_2) : T2) by eauto using msubst_preserves_typing_1.
-    assert (emptyContext |-+ (Apply t4_1 t4_2) : T2) by eauto using msubst_preserves_typing_2.
-
-    assert (R1: RC k (Ty_Fun T1 T2) t3_1 t4_1) by (eapply IH_t1; eauto; apply skip).
-    assert (R2: RC k T1 t3_2 t4_2) by (eapply IH_t2; eauto; apply skip).
-
-    eapply RC_compatibility_Apply; eauto.*)
-    
-  - (* T_Builtin*)
-    apply skip.
-
   - (* T_TyInst *)
     intros.
     unfold P_has_type.
     unfold LR_logically_approximate.
     
     apply skip.
-
-  - (* T_Error *)
-    apply skip.
-
-  - (* T_Unwrap *)
-
-    (*
-    intros Gamma M F K T S Htyp_M IH_M Hkind_T Hbr.
-    unfold P_has_type.
-    intros k c e1 e2 Heq Htyp _ V t2 t3 Hmsubst_t2 Hmsubst_t3.
-
-    unfold P_has_type in IH_M.
-
-    assert (exists M', msubst e1 M M' /\ t2 = Unwrap M')
-      by eauto using msubst_Unwrap.
-    destruct H as [M' [Hmsubst_M' Heq_t2]].
-    subst.
-
-    assert (exists M'', msubst e2 M M'' /\ t3 = Unwrap M'')
-      by eauto using msubst_Unwrap.
-    destruct H as [M'' [Hmsubst_M'' Heq_t3]].
-    subst.
-
-    assert (emptyContext |-+ (Unwrap M') : (beta_reduce (unwrapIFix F K T))) 
-      by eauto using msubst_preserves_typing_1.
-    assert (emptyContext |-+ (Unwrap M'') : (beta_reduce (unwrapIFix F K T)))
-      by eauto using msubst_preserves_typing_2.
-
-    assert (RC k (Ty_IFix F T) M' M''). {
-      eapply IH_M; eauto.
-    }
-
-    eapply RC_compatibility_Unwrap; eauto.
-    + inversion H. subst. apply skip. (* TODO *)
-    *)
-    apply skip.
-Abort.
+  - unfold P_constructor_well_formed. eauto with typing.
+  - unfold P_bindings_well_formed_nonrec. eauto with typing.
+  - unfold P_bindings_well_formed_nonrec. eauto with typing.
+  - unfold P_bindings_well_formed_rec. eauto with typing.
+  - unfold P_bindings_well_formed_rec. eauto with typing.
+  - unfold P_binding_well_formed. eauto with typing.
+  - unfold P_binding_well_formed. eauto with typing.
+  - unfold P_binding_well_formed. eauto with typing. 
+Qed.
